pulse/lib/pulse/lib/pledge/Pulse.Lib.Pledge.fsti
@@ -15,6 +15,7 @@
 *)
 
 module Pulse.Lib.Pledge
+#lang-pulse
 
 open Pulse.Lib.Pervasives
 
@@ -29,73 +30,83 @@ val pledge (is:inames) (f:slprop) (v:slprop) : slprop
 unfold
 let pledge0 (f:slprop) (v:slprop) : slprop = pledge emp_inames f v
 
-val pledge_sub_inv (is1:inames) (is2:inames { inames_subset is1 is2 }) (f v:slprop)
-  : stt_ghost unit emp_inames
-                   (pledge is1 f v)
-                   (fun _ -> pledge is2 f v)
+ghost
+fn pledge_sub_inv (is1:inames) (is2:inames { inames_subset is1 is2 }) (f v:slprop)
+  requires pledge is1 f v
+  ensures pledge is2 f v
 
 (* Anything that holds now holds in the future too. *)
-val return_pledge (f v:slprop)
-  : stt_ghost unit emp_inames v (fun _ -> pledge emp_inames f v)
+ghost
+fn return_pledge (f v:slprop)
+  requires v
+  ensures pledge emp_inames f v
 
-val make_pledge (is:inames) (f:slprop) (v:slprop) (extra:slprop)
+ghost
+fn make_pledge (is:inames) (f:slprop) (v:slprop) (extra:slprop)
   (k:unit -> stt_ghost unit is (f ** extra) (fun _ -> f ** v))
-  : stt_ghost unit emp_inames extra (fun _ -> pledge is f v)
+  requires extra
+  ensures pledge is f v
 
-val redeem_pledge (is:inames) (f v:slprop)
-  : stt_ghost unit is (f ** pledge is f v) (fun () -> f ** v)
+ghost
+fn redeem_pledge (is:inames) (f v:slprop)
+  requires f ** pledge is f v
+  ensures  f ** v
+  opens is
 
-val squash_pledge (is:inames) (f:slprop) (v1:slprop)
-  : stt_ghost unit emp_inames (pledge is f (pledge is f v1)) (fun () -> pledge is f v1)
+ghost
+fn squash_pledge (is:inames) (f:slprop) (v1:slprop)
+  requires pledge is f (pledge is f v1)
+  ensures pledge is f v1
 
 // Unclear how useful/convenient this is
-val bind_pledge (#is:inames) (#f:slprop) (#v1:slprop) (#v2:slprop)
+ghost
+fn bind_pledge (#is:inames) (#f:slprop) (#v1:slprop) (#v2:slprop)
         (extra : slprop)
         (#is_k:inames { inames_subset is_k is })
         (k:unit -> stt_ghost unit is_k (f ** extra ** v1) (fun _ -> f ** pledge is f v2))
-  : stt_ghost unit emp_inames (pledge is f v1 ** extra) (fun _ -> pledge is f v2)
+  requires pledge is f v1 ** extra
+  ensures pledge is f v2
 
 (* Weaker variant, the proof does not use f. It's implemented
 by framing k with f and then using the above combinator. Exposing
 only in case it's useful for inference. *)
-val bind_pledge' (#is:inames) (#f:slprop) (#v1:slprop) (#v2:slprop)
+ghost
+fn bind_pledge' (#is:inames) (#f:slprop) (#v1:slprop) (#v2:slprop)
         (extra : slprop)
         (#is_k:inames { inames_subset is_k is })
         (k:unit -> stt_ghost unit is_k (extra ** v1) (fun _ -> pledge is f v2))
-  : stt_ghost unit emp_inames (pledge is f v1 ** extra) (fun () -> pledge is f v2)
+  requires pledge is f v1 ** extra
+  ensures pledge is f v2
 
-val rewrite_pledge_full (#is:inames) (#f:slprop) (v1 : slprop) (v2 : slprop)
+ghost
+fn rewrite_pledge_full (#is:inames) (#f:slprop) (v1 : slprop) (v2 : slprop)
   (#is_k:inames { inames_subset is_k is })
   (k:unit -> stt_ghost unit is_k (f ** v1) (fun _ -> f ** v2))
-  : stt_ghost unit emp_inames
-      (pledge is f v1)
-      (fun _ -> pledge is f v2)
+  requires pledge is f v1
+  ensures pledge is f v2
 
-val rewrite_pledge (#is:inames) (#f:slprop) (v1 : slprop) (v2 : slprop)
+ghost
+fn rewrite_pledge (#is:inames) (#f:slprop) (v1 : slprop) (v2 : slprop)
   (#is_k:inames { inames_subset is_k is })
   (k:unit -> stt_ghost unit is_k v1 (fun _ -> v2))
-  : stt_ghost unit emp_inames
-      (pledge is f v1)
-      (fun _ -> pledge is f v2)
+  requires pledge is f v1
+  ensures  pledge is f v2
 
-val join_pledge (#is:inames) (#f:slprop) (v1:slprop) (v2:slprop)
-  : stt_ghost unit emp_inames
-      (pledge is f v1 ** pledge is f v2)
-      (fun () -> pledge is f (v1 ** v2))
+ghost
+fn join_pledge (#is:inames) (#f:slprop) (v1:slprop) (v2:slprop)
+  requires pledge is f v1 ** pledge is f v2
+  ensures pledge is f (v1 ** v2)
 
 (* Heterogenous variant. Takes the result invlist as an arg since we don't have
 a join defined yet. *)
-val squash_pledge' (is1 is2 is:inames) (f:slprop) (v1:slprop)
-  : stt_ghost unit emp_inames
-       (pure (inames_subset is1 is) **
-        pure (inames_subset is2 is) **
-        pledge is1 f (pledge is2 f v1))
-       (fun () -> pledge is f v1)
+ghost
+fn squash_pledge' (is1 is2 is:inames) (f:slprop) (v1:slprop)
+  requires pure (inames_subset is1 is) ** pure (inames_subset is2 is) **
+           pledge is1 f (pledge is2 f v1)
+  ensures pledge is f v1
 
-// // NB: This must be an unobservable step, and not ghost,
-// // as it allocates an invariant.
-// // val split_pledge (#is:invlist) (#f:slprop) (v1:slprop) (v2:slprop)
-// //   : stt_ghost (pi:invlist_elem { not (mem_inv (invlist_names is) (snd pi)) })
-// //               (invlist_names is)
-// //               (pledge is f (v1 ** v2))
-// //               (fun pi -> pledge (add_one pi is) f v1 ** pledge (add_one pi is) f v2)
+// This is not ghost as it must buy some later credits.
+fn split_pledge (#is:inames) (#f:slprop) (v1:slprop) (v2:slprop)
+  requires pledge is f (v1 ** v2)
+  returns i : (i : iname { not (mem_inv is i) })
+  ensures pledge (add_inv is i) f v1 ** pledge (add_inv is i) f v2
